proof_check.mli
@@ -5,6 +5,8 @@ module Nat :
  sig
  end
 
+val existsb : ('a1 -> bool) -> 'a1 list -> bool
+
 val forallb : ('a1 -> bool) -> 'a1 list -> bool
 
 module Literal :
