src/Model.v
@@ -1,6 +1,50 @@
-Class FModel := {
-  eval : nat -> bool
-}.
+From Coq Require Import Arith List ListSet.
+Import ListNotations.
 
-Coercion eval : FModel >-> Funclass.
+Ltac nat_eq :=
+  match goal with
+  | [ E : _ =? _ = true |- _ ] =>
+    apply beq_nat_true in E as ->; clear E; nat_eq
+    | [ E : _ =? _ = false |- _ ] =>
+    apply beq_nat_false in E; clear E; nat_eq
+  | _ =>
+    simpl; try (rewrite Nat.eqb_refl in *); simpl; intuition
+  end.
 
+Ltac case_eq m n :=
+  simpl in *; destruct (Nat.eqb m n) eqn:E; nat_eq.
+
+Module Type MODEL.
+  Parameter t : Type.
+  Parameter get : t -> nat -> bool.
+End MODEL.
+
+
+Module LModel <: MODEL.
+
+Definition t := list nat.
+
+Fixpoint get (m : t) (n : nat) :=
+  match m with
+  | [] => false
+  | x::xs =>
+    if x =? n then true
+    else get xs n
+  end.
+
+Lemma In_satisfy :
+  forall m n, In n m <-> get m n = true.
+Proof.
+  intros. induction m. easy. split.
+  + intros [-> | H]; [nat_eq | case_eq a n].
+  + intros. case_eq a n.
+Qed.
+
+End LModel.
+
+
+Definition t := nat -> bool.
+
+Definition get (m : t) n := m n.
+
+Definition inv (m : t) := fun x => negb (m x).
